simplification.v: general cleanup and reciprocal bind rule.
The proof of the reciprocal rule does not yet work because of [CFlip].

coq-osiris/theories/semantics/simplification.v
@@ -4,14 +4,18 @@ From osiris.lang Require Import locations lang.
 From osiris.semantics Require Import code eval step.
 Local Open Scope nat_scope.
 
-(* This file defines a simplification relation: [simplify _ m m'] means that
-   [m] can be simplified to [m'].
+(* This file defines a simplification relation: [simp m m'] means that
+   [m] can be simplified to [m']. Simplification is pure (it does not
+   involve the heap and cannot make non-deterministic choices).
 
    When this relation holds, we expect [WP m' φ] to imply [WP m φ]. This
    means that one can prove a safety property of the simpler program [m']
    and transport this property back to [m].
 
-   The simplification relation can serve two slightly distinct purposes:
+   A simplification step is not necessarily a reduction step: that is,
+   [simplify] is not a subrelation of [step].
+
+   The simplification relation can serve two distinct (but related) purposes:
 
    - It can be used to simplify a program while proving that this program
      satisfies a specification of the form of [WP m φ]. This simplification
@@ -20,44 +24,139 @@ Local Open Scope nat_scope.
    - It can be used to write specifications for pure programs. Indeed, if a
      program is pure (that is, does not involve divergence, non-determinism,
      or mutable state) then it should admit a specification of the form
-     [∃ n a, simplify n m (ret a) ∧ P a].
+     [∃ a, simp m (ret a) ∧ φ a]. See the judgement [total] in this file.
 
-     Such a specification implies [WP m (λa, ⌜ P a ⌝)], so a pure program
+     Such a specification implies [WP m (λa, ⌜ φ a ⌝)], so a pure program
      is a special case of a possibly-impure program. *)
 
 (* -------------------------------------------------------------------------- *)
 
-(* The simplification relation is inductively defined as follows. *)
+(* The relation [simp m m'] is inductively defined as follows. *)
 
-(* The constructors [SimplifyEval] and [SimplifyLoop] allow certain [Stop]
-   events to be replaced with their meaning.
+(* The constructors [SimpEval] and [SimpLoop] allow certain [Stop] events to
+   be replaced with their meaning.
 
-   [SimplifyFlip] requires that the computations [k false] and [k true] can
-   both be simplified to a common computation [m]. Thus, [SimplifyFlip] is
-   applicable only in the special case where the final outcome of the
-   computation is independent of the coin flip. This is useful; e.g., it
-   allows OCaml's [assert] construct to be regarded pure.
+   [SimpFlip] requires that the computations [k false] and [k true] can both
+   be simplified to a common computation [m]. Thus, [SimpFlip] is applicable
+   only in the special case where the final outcome of the computation is
+   independent of the coin flip. This is useful; e.g., it allows OCaml's
+   [assert] construct to be regarded pure.
 
-   Two constructors [SimplifyParRetLeft] and [SimplifyParRetRight] simplify a
-   [par] construct where at least one side is [ret _].
+   Two constructors [SimpParRetLeft] and [SimpParRetRight] simplify a [par]
+   construct where at least one side is [ret _].
 
-   A simplification step is not necessarily a reduction step: that is,
-   [simplify] is not a subrelation of [step].
+   The constructor [SimpPar] allows simplification to take place under a [Par]
+   constructor.
 
-   The constructor [SimplifyPar] allows simplification to take place under a
-   [Par] constructor.
+   The constructors [SimpReflexive] and [SimpTransitive] make simplification
+   reflexive and transitive by definition. This is essentially forced on us,
+   because otherwise the premises of [SimpFlip] would be too restrictive. The
+   paths from [k false] to [m] and from [k true] to [m] must be allowed to
+   have different lengths. *)
 
-   The constructors [SimplifyReflexive] and [SimplifyTransitive] make
-   simplification reflexive and transitive by definition. This is essentially
-   forced on us, because otherwise the premises of [SimplifyFlip] would be too
-   restrictive. The paths from [k false] to [m] and from [k true] to [m] must
-   be allowed to have different lengths. *)
+Inductive simp {A : Type} : micro A → micro A → Prop :=
+| SimpEval:
+    ∀ η e k ko,
+    simp
+      (Stop CEval (η, e) k ko)
+      (try (eval η e) k ko)
+| SimpLoop :
+    ∀ η x i1 i2 e k ko,
+    simp
+      (Stop CLoop (η, x, i1, i2, e) k ko)
+      (try (loop η x i1 i2 e) k ko)
+| SimpFlip :
+    ∀ x k ko m,
+    simp (k false) m →
+    simp (k true) m →
+    simp
+      (Stop CFlip x k ko)
+      m
+| SimpParRetLeft:
+    ∀ {A1 A2} (a1 : A1) (m2 : micro A2) k ko,
+    simp
+      (Par (Ret a1) m2 k ko)
+      (try m2 (λ v2, k (a1, v2)) ko)
+| SimpParRetRight:
+    ∀ {A1 A2} (m1 : micro A1) (a2 : A2) k ko,
+    simp
+      (Par m1 (Ret a2) k ko)
+      (try m1 (λ v1, k (v1, a2)) ko)
+| SimpPar:
+    ∀ {A1 A2} m1 m'1 m2 m'2 (k : A1 * A2 → micro A) ko,
+    simp m1 m'1 →
+    simp m2 m'2 →
+    simp (Par m1 m2 k ko) (Par m'1 m'2 k ko)
+| SimpReflexive:
+    ∀ m,
+    simp m m
+| SimpTransitive:
+    ∀ m1 m2 m3,
+    simp m1 m2 →
+    simp m2 m3 →
+    simp m1 m3
+.
 
-(* The relation [simplify n m m'] is indexed with a natural integer [n], which
-   measures the length of the simplification path. The main simulation lemmas,
-   [simplify_step_diagram] and [simplify_ret_step_diagram], control the manner
+Global Hint Constructors simp : simp.
+
+(* -------------------------------------------------------------------------- *)
+
+(* More (derived) construction rules for [simp]. *)
+
+(* The following two auxiliary lemmas can be useful when a constructor cannot
+   be applied directly. *)
+
+Lemma simp_up_to_eq_left {A} {m1 m1' m2 : micro A} :
+  simp m1' m2 →
+  m1 = m1' →
+  simp m1 m2.
+Proof.
+  congruence.
+Qed.
+
+Lemma simp_up_to_eq_right {A} {m1 m2 m2' : micro A} :
+  simp m1 m2 →
+  m2 = m2' →
+  simp m1 m2'.
+Proof.
+  congruence.
+Qed.
+
+(* Derived constructors. *)
+
+Lemma SimpParRetRet {A1 A2 A} a1 a2 (k : A1 * A2 → micro A) ko :
+  simp
+    (Par (Ret a1) (Ret a2) k ko)
+    (k (a1, a2)).
+Proof.
+  eauto using simp_up_to_eq_right with simp try_ret.
+Qed.
+
+Lemma SimpParRetLeftNext {A1 A2 A} a1 m2 (k : A1 * A2 → micro A) :
+  simp
+    (Par (Ret a1) m2 k next)
+    (v2 ← m2 ; k (a1, v2)).
+Proof.
+  eauto using simp_up_to_eq_right with simp bind_as_try.
+Qed.
+
+Lemma SimpParRetRightNext {A1 A2 A} m1 a2 (k : A1 * A2 → micro A) :
+  simp
+    (Par m1 (Ret a2) k next)
+    (v1 ← m1 ; k (v1, a2)).
+Proof.
+  eauto using simp_up_to_eq_right with simp bind_as_try.
+Qed.
+
+(* -------------------------------------------------------------------------- *)
+
+(* We define a 3-argument relation [simplify n m m'] where the natural integer
+   [n] measures the length of the simplification path. The simulation lemmas
+   [simplify_step_diagram] and [simplify_ret_step_diagram] control the manner
    in which [n] decreases or is preserved. This is necessary for the proof of
    the lemma [wp_simplify] to go through. *)
+
+(* End users need not be know about this relation. *)
 
 Inductive simplify {A : Type} : nat → micro A → micro A → Prop :=
 | SimplifyEval:
@@ -108,6 +207,39 @@ Inductive simplify {A : Type} : nat → micro A → micro A → Prop :=
 
 Global Hint Constructors simplify : simplify.
 
+(* -------------------------------------------------------------------------- *)
+
+(* [simplify _ m m'] and [simp m m'] are equivalent. *)
+
+(* [simplify n m1 m2] implies [simp m1 m2]. *)
+
+Lemma simplify_simp {A} n (m1 m2 : micro A) :
+  simplify n m1 m2 →
+  simp m1 m2.
+Proof.
+  induction 1; intros; subst; eauto with simp.
+Qed.
+
+(* [simp m1 m2] implies [simplify n m1 m2] for some [n]. *)
+
+Lemma simp_simplify {A} {m1 m2 : micro A} :
+  simp m1 m2 →
+  ∃ n,
+  simplify n m1 m2.
+Proof.
+  induction 1;
+  repeat match goal with h: ∃ n, _ |- _ => destruct h end;
+  eauto using
+    (SimplifyEval 0),
+    (SimplifyLoop 0),
+    (SimplifyParRetLeft 0),
+    (SimplifyParRetRight 0),
+    (SimplifyReflexive 0)
+    with simplify.
+Qed.
+
+(* -------------------------------------------------------------------------- *)
+
 (* Simplification is compatible with [try]. *)
 
 Lemma simplify_try {A B} n (m1 m2 : micro A) (f : A → micro B) ko :
@@ -118,6 +250,14 @@ Proof.
   rewrite ?try_try; econstructor; eauto with congruence.
 Qed.
 
+Lemma simp_try {A B} (m1 m2 : micro A) (f : A → micro B) ko :
+  simp m1 m2 →
+  simp (try m1 f ko) (try m2 f ko).
+Proof.
+  induction 1; simpl; rewrite ?try_try;
+  econstructor; eauto with congruence.
+Qed.
+
 (* Simplification is compatible with [bind]. *)
 
 Lemma simplify_bind {A B} n (m1 m2 : micro A) (f : A → micro B) :
@@ -125,6 +265,13 @@ Lemma simplify_bind {A B} n (m1 m2 : micro A) (f : A → micro B) :
   simplify n (bind m1 f) (bind m2 f).
 Proof.
   rewrite !bind_as_try. eauto using simplify_try.
+Qed.
+
+Lemma simp_bind {A B} (m1 m2 : micro A) (f : A → micro B) :
+  simp m1 m2 →
+  simp (bind m1 f) (bind m2 f).
+Proof.
+  rewrite !bind_as_try. eauto using simp_try.
 Qed.
 
 (* -------------------------------------------------------------------------- *)
@@ -140,10 +287,24 @@ Proof.
   intro h; dependent induction h; eauto.
 Qed.
 
+Lemma destruct_simp_ret {A} a1 (m2 : micro A) :
+  simp (ret a1) m2 →
+  m2 = ret a1.
+Proof.
+  intro h; dependent induction h; eauto.
+Qed.
+
 (* [crash] cannot be simplified. *)
 
 Lemma destruct_simplify_crash {A} n (m2 : micro A) :
   simplify n crash m2 →
+  m2 = crash.
+Proof.
+  intro h; dependent induction h; eauto.
+Qed.
+
+Lemma destruct_simp_crash {A} (m2 : micro A) :
+  simp crash m2 →
   m2 = crash.
 Proof.
   intro h; dependent induction h; eauto.
@@ -158,13 +319,27 @@ Proof.
   intro h; dependent induction h; eauto.
 Qed.
 
-(* This tactic applies the above lemmas if possible. *)
+Lemma destruct_simp_next {A} (m2 : micro A) :
+  simp Next m2 →
+  m2 = Next.
+Proof.
+  intro h; dependent induction h; eauto.
+Qed.
+
+(* These tactics apply the above lemmas, if possible. *)
 
 Ltac clarify_simplify :=
   repeat match goal with
   | h: simplify _ (ret _) ?m |- _ => apply destruct_simplify_ret in h
   | h: simplify _ crash ?m |- _ => apply destruct_simplify_crash in h
   | h: simplify _ Next ?m |- _ => apply destruct_simplify_next in h
+  end; simplify_eq.
+
+Ltac clarify_simp :=
+  repeat match goal with
+  | h: simp (ret _) ?m |- _ => apply destruct_simp_ret in h
+  | h: simp crash ?m |- _ => apply destruct_simp_crash in h
+  | h: simp Next ?m |- _ => apply destruct_simp_next in h
   end; simplify_eq.
 
 (* -------------------------------------------------------------------------- *)
@@ -466,9 +641,8 @@ Qed.
 (* This result is stronger than [simplify_ret_confluent], because not
    every computation can be simplified to [ret _]. *)
 
-(* This lemma is currently unused. Nevertheless, I have spent a couple
-   hours proving it, mostly as a challenge for myself, so I am keeping
-   it. *)
+(* This lemma is not crucial. Nevertheless, I have spent a couple hours
+   proving it, mostly as a challenge for myself, so I am keeping it. *)
 
 Lemma simplify_confluent :
   ∀ {n i2 j' A} {m1 m2 m'1 : micro A},
@@ -540,119 +714,9 @@ Proof.
   ].
 Qed.
 
-(* -------------------------------------------------------------------------- *)
-
-(* A non-indexed simplification relation. *)
-
-(* This version is intended for use by end users. *)
-
-Inductive simp {A : Type} : micro A → micro A → Prop :=
-| SimpEval:
-    ∀ η e k ko,
-    simp
-      (Stop CEval (η, e) k ko)
-      (try (eval η e) k ko)
-| SimpLoop :
-    ∀ η x i1 i2 e k ko,
-    simp
-      (Stop CLoop (η, x, i1, i2, e) k ko)
-      (try (loop η x i1 i2 e) k ko)
-| SimpFlip :
-    ∀ x k ko m,
-    simp (k false) m →
-    simp (k true) m →
-    simp
-      (Stop CFlip x k ko)
-      m
-| SimpParRetLeft:
-    ∀ {A1 A2} (a1 : A1) (m2 : micro A2) k ko,
-    simp
-      (Par (Ret a1) m2 k ko)
-      (try m2 (λ v2, k (a1, v2)) ko)
-| SimpParRetRight:
-    ∀ {A1 A2} (m1 : micro A1) (a2 : A2) k ko,
-    simp
-      (Par m1 (Ret a2) k ko)
-      (try m1 (λ v1, k (v1, a2)) ko)
-| SimpPar:
-    ∀ {A1 A2} m1 m'1 m2 m'2 (k : A1 * A2 → micro A) ko,
-    simp m1 m'1 →
-    simp m2 m'2 →
-    simp (Par m1 m2 k ko) (Par m'1 m'2 k ko)
-| SimpReflexive:
-    ∀ m,
-    simp m m
-| SimpTransitive:
-    ∀ m1 m2 m3,
-    simp m1 m2 →
-    simp m2 m3 →
-    simp m1 m3
-.
-
-Global Hint Constructors simp : simp.
-
-(* This auxiliary lemma is useful when a constructor of the relation [simp]
-   cannot be applied directly. *)
-
-Lemma simp_up_to_eq {A} {m1 m2 m2' : micro A} :
-  simp m1 m2 →
-  m2 = m2' →
-  simp m1 m2'.
-Proof.
-  congruence.
-Qed.
-
-(* Simplification is compatible with [try]. *)
-
-Lemma simp_try {A B} (m1 m2 : micro A) (f : A → micro B) ko :
-  simp m1 m2 →
-  simp (try m1 f ko) (try m2 f ko).
-Proof.
-  induction 1; simpl; rewrite ?try_try;
-  econstructor; eauto with congruence.
-Qed.
-
-(* Simplification is compatible with [bind]. *)
-
-Lemma simp_bind {A B} (m1 m2 : micro A) (f : A → micro B) :
-  simp m1 m2 →
-  simp (bind m1 f) (bind m2 f).
-Proof.
-  rewrite !bind_as_try. eauto using simp_try.
-Qed.
-
-(* [simplify n m1 m2] implies [simp m1 m2]. *)
-
-(* This property should not be needed, but is a sanity check. *)
-
-Lemma simplify_simp {A} n (m1 m2 : micro A) :
-  simplify n m1 m2 →
-  simp m1 m2.
-Proof.
-  induction 1; intros; subst; eauto with simp.
-Qed.
-
-(* [simp m1 m2] implies [simplify n m1 m2] for some [n]. *)
-
-Lemma simp_simplify {A} {m1 m2 : micro A} :
-  simp m1 m2 →
-  ∃ n,
-  simplify n m1 m2.
-Proof.
-  induction 1;
-  repeat match goal with h: ∃ n, _ |- _ => destruct h end;
-  eauto using
-    (SimplifyEval 0),
-    (SimplifyLoop 0),
-    (SimplifyParRetLeft 0),
-    (SimplifyParRetRight 0),
-    (SimplifyReflexive 0)
-    with simplify.
-Qed.
-
 (* The relation [simp _ (ret _)] is confluent. *)
 
-Lemma simp_ret_confluent {A} (m : micro A) a1 a2 :
+Lemma simp_ret_confluent {A} {m : micro A} {a1 a2} :
   simp m (ret a1) →
   simp m (ret a2) →
   a1 = a2.
@@ -663,9 +727,15 @@ Proof.
   eauto using simplify_ret_confluent.
 Qed.
 
+Ltac simp_ret_confluent :=
+  match goal with
+  | h1: simp ?m (ret ?a1), h2: simp ?m (ret ?a2) |- _ =>
+      generalize (simp_ret_confluent h1 h2); intro
+  end.
+
 (* The relation [simp] is confluent. *)
 
-Lemma simp_confluent {A} (m1 m2 m'1 : micro A) :
+Lemma simp_confluent {A} {m1 m2 m'1 : micro A} :
   simp m1 m2 →
   simp m1 m'1 →
   ∃ m'2,
@@ -680,35 +750,15 @@ Proof.
   eauto using simplify_simp.
 Qed.
 
-(* Special cases. *)
-
-Lemma SimpParRetRet {A1 A2 A} a1 a2 (k : A1 * A2 → micro A) ko :
-  simp
-    (Par (Ret a1) (Ret a2) k ko)
-    (k (a1, a2)).
-Proof.
-  eauto using simp_up_to_eq with simp try_ret.
-Qed.
-
-Lemma SimpParRetLeftNext {A1 A2 A} a1 m2 (k : A1 * A2 → micro A) :
-  simp
-    (Par (Ret a1) m2 k next)
-    (v2 ← m2 ; k (a1, v2)).
-Proof.
-  eauto using simp_up_to_eq with simp bind_as_try.
-Qed.
-
-Lemma SimpParRetRightNext {A1 A2 A} m1 a2 (k : A1 * A2 → micro A) :
-  simp
-    (Par m1 (Ret a2) k next)
-    (v1 ← m1 ; k (v1, a2)).
-Proof.
-  eauto using simp_up_to_eq with simp bind_as_try.
-Qed.
+Ltac simp_confluent :=
+  match goal with
+  | h1: simp ?m ?m'1, h2: simp ?m ?m'2 |- _ =>
+      generalize (simp_confluent h1 h2)
+  end.
 
 (* -------------------------------------------------------------------------- *)
 
-(* Useful typeclass instances. *)
+(* Useful type class instances. *)
 
 (* Instantiating [Reflexive] allows to use [reflexivity] to prove
    [simp ?m ?m]. *)
@@ -719,3 +769,541 @@ Global Instance TC_reflexivity_simp {A} : Reflexive (@simp A) :=
    [etransitivity] to prove [simp ?m ?m']. *)
 Global Instance TC_transitivity_simp {A} : Transitive (@simp A) :=
   SimpTransitive.
+
+(* -------------------------------------------------------------------------- *)
+
+(* We now define a Hoare logic for pure expressions. *)
+
+(* Because this definition is based on [simp], it can be used to reason about
+   pure expressions only. Because [simp] is inductively defined, it can reason
+   about terminating expressions only; it is a logic of total correctness. *)
+
+(* This Hoare logic can reason both about expressions that terminate normally
+   and about expressions that raise the exception [Next]. *)
+
+(* The judgement [total m φ ψ] means that either [m] terminates and produces
+   a value [a] that satisfies the postcondition [φ], or [m] raises [Next],
+   in which case [ψ] is satisfied. *)
+
+Definition total {A} m (φ : A → Prop) ψ :=
+  (∃ a, simp m (ret a) ∧ φ a) ∨
+  (simp m Next ∧ ψ).
+
+Ltac destruct_total :=
+  match goal with
+  | h: total _ _ _ |- _ =>
+      destruct h as [ (? & ? & ?) | (? & ?) ]
+  end.
+
+(* The reasoning rule for [ret _]. *)
+
+Lemma total_ret {A} a (φ : A → Prop) ψ :
+  φ a →
+  total (ret a) φ ψ.
+Proof.
+  intros. left. eauto with simp.
+Qed.
+
+(* The reasoning rule for [Next]. *)
+
+Lemma total_Next {A} (φ : A → Prop) (ψ : Prop) :
+  ψ →
+  total Next φ ψ.
+Proof.
+  intros. right. eauto with simp.
+Qed.
+
+(* The consequence rule. *)
+
+Lemma total_consequence {A} m (φ φ' : A → Prop) (ψ ψ' : Prop) :
+  total m φ ψ →
+  (∀ a, φ a → φ' a) →
+  (ψ → ψ') →
+  total m φ' ψ'.
+Proof.
+  intros. destruct_total.
+  { left. eauto. }
+  { right. eauto. }
+Qed.
+
+(* The simplification rule. *)
+
+(* This rule allows performing a simplification step in the middle
+   of a Hoare-style proof. *)
+
+(* Although there is no reasoning rule for [Stop], the lemma [total_simp] can
+   be used to reason about [Stop CEval] and [Stop CLoop]. *)
+
+Lemma total_simp {A} m m' (φ : A → Prop) (ψ : Prop) :
+  simp m m' →
+  total m' φ ψ →
+  total m φ ψ.
+Proof.
+  intros. destruct_total.
+  { left. eauto with simp. }
+  { right. eauto with simp. }
+Qed.
+
+(* A reasoning rule for [try]. *)
+
+Lemma total_try {A B} m f g (φ : B → Prop) (φ' : A → Prop) (ψ ψ' : Prop) :
+  total m φ' ψ' →
+  (∀ a, φ' a → total (f a) φ ψ) →
+  (ψ' → total (g ()) φ ψ) →
+  total (try m f g) φ ψ.
+Proof.
+  intros. destruct_total.
+  { eapply total_simp; [ eapply simp_try; eauto |].
+    rewrite try_ret.
+    eauto. }
+  { eapply total_simp; [ eapply simp_try; eauto |].
+    rewrite try_next.
+    eauto. }
+Qed.
+
+(* A reasoning rule for [bind]. *)
+
+Lemma total_bind {A B} m f (φ : B → Prop) (φ' : A → Prop) (ψ : Prop) :
+  total m φ' ψ →
+  (∀ a, φ' a → total (f a) φ ψ) →
+  total (bind m f) φ ψ.
+Proof.
+  rewrite bind_as_try. eauto using total_try, total_Next.
+Qed.
+
+Lemma total_bind_unary {A B} m f (φ : B → Prop) (ψ : Prop) :
+  total m (λ (a : A), total (f a) φ ψ) ψ →
+  total (bind m f) φ ψ.
+Proof.
+  eauto using total_bind.
+Qed.
+
+(* A reasoning rule for [par]. *)
+
+(* This rule is limited to the case where [ψ] is [False] because dealing with
+   arbitrary [ψ] would require the ability to simplify [Par Next Next _ _]
+   into [Next]. The relation [simp] currently does not allow this. *)
+
+Lemma total_par {A1 A2} m1 m2
+  (φ1 : A1 → Prop) (φ2 : A2 → Prop) (φ : A1 * A2 → Prop)
+:
+  let ψ := False in
+  total m1 φ1 ψ →
+  total m2 φ2 ψ →
+  (∀ a1 a2, φ1 a1 ∧ φ2 a2 → φ (a1, a2)) →
+  total (par m1 m2) φ ψ.
+Proof.
+  intros. repeat destruct_total.
+  { eapply total_simp.
+    eapply SimpPar; eassumption.
+    eapply total_simp; [ eapply SimpParRetRet |].
+    eapply total_ret.
+    eauto. }
+  { eapply total_simp.
+    eapply SimpPar; eassumption.
+    eapply total_simp; [ eapply SimpParRetRight |].
+    rewrite try_next.
+    eapply total_Next.
+    eauto. }
+  { eapply total_simp.
+    eapply SimpPar; eassumption.
+    eapply total_simp; [ eapply SimpParRetLeft |].
+    rewrite try_next.
+    eapply total_Next.
+    eauto. }
+  { exfalso. tauto. }
+Qed.
+
+(* The infinitary intersection rule. *)
+
+(* If for every [x] one can prove that the result of [m] satisfies [φ x],
+   then one can deduce that the result of [m] satisfies [φ x] for every
+   [x] simultaneously. *)
+
+Lemma total_intersection {A} `{Inhabited X} m (φ : X → A → Prop) (ψ : Prop) :
+  (∀ x, total m (φ x) ψ) →
+  total m (λ a, ∀ x, φ x a) ψ.
+Proof.
+  intros Hm.
+  (* Instantiate [Hm] with an arbitrary [x]. *)
+  generalize (Hm inhabitant). intros [ (a & ? & ?) | (? & ?) ].
+  (* Case: there exists [a] such that [m] can be simplified to [ret a]. *)
+  { left. exists a. split; [ eauto |].
+    intros x. destruct (Hm x) as [ (a' & ? & ?) | (? & ?) ].
+    (* Because [simp _ (ret _)] is confluent, [a] and [a'] must be equal. *)
+    { simp_ret_confluent. congruence. }
+    (* Because [simp _ _] is confluent, [m] cannot be simplified both to
+       [ret _] and [Next]. So, this subcase is impossible. *)
+    { exfalso. simp_confluent; intros (m' & h1 & h2). clarify_simp. }
+  }
+  (* Case: [m] can be simplified to [Next]. *)
+  { right. eauto. }
+Qed.
+
+(* The binary intersection rule. *)
+
+(* If one can prove that the result of [m] satisfies [φ1]
+   and if one can prove that the result of [m] satisfies [φ2]
+   then one can deduce that the result of [m] satisfies [φ1] and [φ2]
+   simultaneously. *)
+
+Lemma total_binary_intersection {A} m (φ1 φ2 : A → Prop) (ψ : Prop) :
+  total m φ1 ψ →
+  total m φ2 ψ →
+  total m (λ a, φ1 a ∧ φ2 a) ψ.
+Proof.
+  intros.
+  set (post := λ (b : bool), λ a, if b then φ1 a else φ2 a).
+  eapply total_consequence with (φ := λ a, ∀ b, post b a) (ψ := ψ).
+  { eapply total_intersection.
+    intros b. destruct b; unfold post; assumption. }
+  { intros a Hpost. split.
+    + apply (Hpost true).
+    + apply (Hpost false). }
+  { tauto. }
+Qed.
+
+(* -------------------------------------------------------------------------- *)
+
+(* We now prepare to prove the reciprocal bind rule, that is,
+   the reverse implication of the lemma [total_bind_unary]. *)
+
+(* -------------------------------------------------------------------------- *)
+
+(* To do so, we need another indexed variant of the relation [simp].
+   This variant places a weight of 1 on every node. This weight is
+   used to do a well-founded induction in the proof of the lemma
+   [invert_stack_try_ret]. *)
+
+(* One can think of a proof of [sss n m m'] as a simplification tree
+   from [m] to [m'] whose weight is [n]. *)
+
+Inductive sss {A : Type} : nat → micro A → micro A → Prop :=
+| SssEval:
+    ∀ p η e k ko,
+    p = (η, e) →
+    sss 1
+      (Stop CEval p k ko)
+      (try (eval η e) k ko)
+| SssLoop :
+    ∀ p η x i1 i2 e k ko,
+    p = (η, x, i1, i2, e) →
+    sss 1
+      (Stop CLoop p k ko)
+      (try (loop η x i1 i2 e) k ko)
+| SssParRetLeft:
+    ∀ {A1 A2} (a1 : A1) (m2 : micro A2) k ko,
+    sss 1
+      (Par (Ret a1) m2 k ko)
+      (try m2 (λ v2, k (a1, v2)) ko)
+| SssParRetRight:
+    ∀ {A1 A2} (m1 : micro A1) (a2 : A2) k ko,
+    sss 1
+      (Par m1 (Ret a2) k ko)
+      (try m1 (λ v1, k (v1, a2)) ko)
+| SssPar:
+    ∀ {A1 A2} n1 n2 n m1 m'1 m2 m'2 (k : A1 * A2 → micro A) ko,
+    sss n1 m1 m'1 →
+    sss n2 m2 m'2 →
+    n1 + n2 ≤ n →
+    sss n (Par m1 m2 k ko) (Par m'1 m'2 k ko)
+| SssReflexive:
+    ∀ m,
+    sss 1 m m
+| SssTransitive:
+    ∀ n1 n2 n m1 m2 m3,
+    sss n1 m1 m2 →
+    sss n2 m2 m3 →
+    n1 + n2 < n →
+    sss n m1 m3
+.
+
+Local Hint Constructors sss : sss.
+
+(* -------------------------------------------------------------------------- *)
+
+(* [sss _ m m'] and [simp m m'] are equivalent. *)
+
+Local Lemma sss_simp {A} {n} {m m' : micro A} :
+  sss n m m' →
+  simp m m'.
+Proof.
+  induction 1; subst; eauto with simp.
+Qed.
+
+Local Lemma simp_sss {A} {m m' : micro A} :
+  simp m m' →
+  ∃ n, sss n m m'.
+Local Ltac baz :=
+  match goal with h: ∃ n, sss n _ _ |- _ => destruct h end.
+Proof.
+  induction 1; try solve [ repeat baz; eauto with lia sss ].
+  (* The case of [CFlip] does not work. *)
+  admit.
+Admitted.
+
+(* -------------------------------------------------------------------------- *)
+
+(* The weight of a simplification tree is positive. *)
+
+Local Lemma sss_positive {A} {n} {m m' : micro A} :
+  sss n m m' →
+  0 < n.
+Proof.
+  induction 1; eauto with lia.
+Qed.
+
+Local Ltac sss_positive :=
+  match goal with h: sss _ _ _ |- _ =>
+    generalize (sss_positive h); intro
+  end.
+
+(* -------------------------------------------------------------------------- *)
+
+(* A stack of simplification trees is needed in the statement of the lemma
+   [invert_stack_try_ret]. *)
+
+(* One can think of this stack as an evaluation context. Although there is
+   no syntax for evaluation contexts, because the [micro] monad is a shallow
+   embedding, making evaluation contexts explicit, and controlling their
+   weight, is required here. *)
+
+Inductive stack {A : Type} : nat → micro A → micro A → Prop :=
+| StackNil:
+    forall n m,
+    0 ≤ n →
+    stack n m m
+| StackCons:
+    forall n1 n2 n m1 m2 m3,
+    sss n1 m1 m2 →
+    stack n2 m2 m3 →
+    n1 + n2 ≤ n →
+    stack n m1 m3.
+
+Local Hint Constructors stack : stack.
+
+(* -------------------------------------------------------------------------- *)
+
+(* In [stack n m m'], the parameter [n] is an over-approximation of the
+   weight of the stack, which itself is the sum of the weights of the
+   trees in the stack. *)
+
+Local Lemma stack_monotone {A} n (m m' : micro A) :
+  ∀ n',
+  stack n m m' →
+  n ≤ n' →
+  stack n' m m'.
+Proof.
+  induction 1; intros; econstructor; eauto with lia.
+Qed.
+
+(* A single tree forms a stack (of one cell). *)
+
+Lemma sss_stack {A} n (m m' : micro A) :
+  sss n m m' →
+  stack n m m'.
+Proof.
+  eauto with stack lia.
+Qed.
+
+(* A stack represents a simplification path. *)
+
+Lemma stack_simp {A} {n} {m m' : micro A} :
+  stack n m m' →
+  simp m m'.
+Proof.
+  induction 1; eauto using sss_simp with simp.
+Qed.
+
+(* -------------------------------------------------------------------------- *)
+
+(* The main lemma. *)
+
+(* If [try m m ko] can be simplified to [ret b]
+   via a stack of weight [n],
+   then:
+   - either [m] can be simplified to [ret a]
+     for some [a] such that
+     [k a] can be simplified to [ret b]
+     via a stack of weight [n],
+   - or [m] can be simplified to [Next]
+     and [ko()] can be simplified to [ret b]
+     via a stack of weight [n].
+ *)
+
+Lemma invert_stack_try_ret :
+  ∀ n {A B} m (k : A → micro B) ko b,
+  stack n (try m k ko) (ret b) →
+  total m
+    (λ a, stack n (k a) (ret b))
+    (stack n (ko()) (ret b)).
+Proof.
+  induction n as [n IH] using (well_founded_induction lt_wf).
+
+  (* Reformulate the induction hypothesis by weakening it so that its
+     conclusion mentions [n] instead of [i]. Also, place the side
+     condition [i < n] in the last position. *)
+  assert (IHw :
+    ∀ i {A B} m (k : A → micro B) ko b,
+    stack i (try m k ko) (ret b) →
+    i < n →
+    total m
+      (λ a, stack n (k a) (ret b))
+      (stack n (ko()) (ret b))
+  ).
+  { intros. eapply total_consequence; intuition eauto using stack_monotone. }
+  clear IH.
+
+  (* Now begin the proof. *)
+  intros A B m k ko b.
+  intros Hstack.
+
+  (* If [m] is [ret a] or [Next], then the result is immediate. Treat
+     these two cases now, so as to avoid treating them several times
+     later on. *)
+  destruct (ret_or_next_or_else m) as [ (a & ?) | [ ? | (Hret & HNext) ]].
+  (* Case: [m] is [ret a]. *)
+  { subst m. rewrite try_ret in Hstack. eapply total_ret. eauto. }
+  (* Case: [m] is [Next]. *)
+  { subst m. rewrite try_next in Hstack. eapply total_Next. eauto. }
+  (* We can now assume that [m] is neither [ret _] nor [Next]. *)
+
+  (* Is the stack empty? *)
+  dependent destruction Hstack.
+  (* Case: the stack is empty. *)
+  { clear IHw. exfalso. eauto using invert_try_eq_ret. }
+  (* Case: the stack is nonempty. Analyze its first element. *)
+  match goal with h: sss _ _ _ |- _ => dependent destruction h end.
+
+  (* Subcase: [SssEval]. *)
+  { subst p.
+    (* [m] is [Stop CEval _ _ _]. *)
+    invert_try_eq_stop. subst m. clear Hret HNext.
+    (* Perform one step forward in the goal. *)
+    eapply total_simp; [eapply SimpEval |].
+    (* Recognize [(try (try _ _ _) _ _)] in the stack. (Yes!) *)
+    rewrite <- try_try in Hstack.
+    (* Abstract away the inner [try _ _ _]. (Optional.) *)
+    match type of Hstack with context[try ?m _ _] =>
+      generalize dependent m
+    end; intros m Hstack.
+    (* We recognize an opportunity to apply the induction hypothesis. *)
+    eauto with lia.
+  }
+
+  (* Subcase: [SssLoop]. *)
+  { subst p.
+    (* [m] is [Stop Loop _ _ _]. *)
+    invert_try_eq_stop. subst m. clear Hret HNext.
+    (* Perform one step forward in the goal. *)
+    eapply total_simp; [eapply SimpLoop |].
+    (* Recognize [(try (try _ _ _) _ _)] in the stack. (Yes!) *)
+    rewrite <- try_try in Hstack.
+    (* Abstract away the inner [try _ _ _]. (Optional.) *)
+    match type of Hstack with context[try ?m _ _] =>
+      generalize dependent m
+    end; intros m Hstack.
+    (* We recognize an opportunity to apply the induction hypothesis. *)
+    eauto with lia.
+  }
+
+  (* Subcase: [SssParRetLeft]. *)
+  {
+    (* [m] is [Par m1 m2 _ _]. *)
+    invert_try_eq_par. subst m. clear Hret HNext.
+    (* Perform one step forward in the goal. *)
+    eapply total_simp; [eapply SimpParRetLeft |].
+    (* Recognize [(try (try _ _ _) _ _)] in the stack. (Yes!) *)
+    rewrite <- try_try in Hstack.
+    (* Apply the induction hypothesis. *)
+    eauto with lia.
+  }
+
+  (* Subcase: [SssParRetRight]. *)
+  {
+    (* [m] is [Par m1 m2 _ _]. *)
+    invert_try_eq_par. subst m. clear Hret HNext.
+    (* Perform one step forward in the goal. *)
+    eapply total_simp; [eapply SimpParRetRight |].
+    (* Recognize [(try (try _ _ _) _ _)] in the stack. (Yes!) *)
+    rewrite <- try_try in Hstack.
+    (* Apply the induction hypothesis. *)
+    eauto with lia.
+  }
+
+  (* Subcase: [SssPar]. *)
+  {
+    (* [m] is [Par m1 m2 _ _]. *)
+    invert_try_eq_par. subst m. clear Hret HNext.
+    (* Change [m1] to [m'1] and [m2] to [m'2] in the goal. *)
+    eapply total_simp.
+    { eapply SimpPar; eapply sss_simp; eauto. }
+    (* Recognize [try (Par _ _ _ _) _ _] in the stack. *)
+    rewrite <- try_par in Hstack.
+    (* Apply the induction hypothesis. *)
+    sss_positive. eauto with lia.
+  }
+
+  (* Subcase: [SssReflexive]. *)
+  { eauto with lia. }
+
+  (* Subcase: [SssTransitive]. *)
+  { eauto with stack lia. }
+
+Qed.
+
+(* -------------------------------------------------------------------------- *)
+
+(* The previous lemma can now be specialized to the case where the stack
+   initially has height one, that is, it consists of a single tree. *)
+
+(* This yields the reciprocal try rule. *)
+
+Lemma invert_simp_try_ret {A B} m (k : A → micro B) ko b :
+  simp (try m k ko) (ret b) →
+  total m
+    (λ a, simp (k a) (ret b))
+    (simp (ko()) (ret b)).
+Proof.
+  intros Hsimp.
+  (* Transform [simp _ _] into [sss n _ _] for some unknown [n]. *)
+  apply simp_sss in Hsimp.
+  destruct Hsimp as (n & Hsimp).
+  (* Thus, we have a stack (of one cell). *)
+  apply sss_stack in Hsimp.
+  (* We can apply the previous lemma. *)
+  apply invert_stack_try_ret in Hsimp.
+  (* The result then follows via the consequence rule. *)
+  eapply total_consequence; [ eauto | |].
+  + simpl. eauto using stack_simp.
+  + eauto using stack_simp.
+Qed.
+
+(* The previous lemma can be specialized to obtain a result about [bind]. *)
+
+Lemma invert_simp_bind_ret_total {A B} m (k : A → micro B) b :
+  simp (bind m k) (ret b) →
+  total m
+    (λ a, simp (k a) (ret b))
+    False.
+Proof.
+  rewrite bind_as_try.
+  intros h.
+  eapply total_consequence.
+  { eauto using invert_simp_try_ret. }
+  { eauto. }
+  (* There remains to argue that [Next] cannot reduce to [ret _]. *)
+  { simpl. intros. clarify_simp. }
+Qed.
+
+(* Unfolding [total] in the previous result yields this perhaps more
+   readable statement. *)
+
+(* This is the reciprocal bind rule. *)
+
+Lemma invert_simp_bind_ret {A B} m (k : A → micro B) b :
+  simp (bind m k) (ret b) →
+  ∃ a, simp m (ret a) ∧ simp (k a) (ret b).
+Proof.
+  intros h. apply invert_simp_bind_ret_total in h. unfold total in h. tauto.
+Qed.
